<?xml version="1.0"?>
<rdf:RDF xmlns:rdf="http://www.w3.org/1999/02/22-rdf-syntax-ns#"
         xmlns:xsd="http://www.w3.org/2001/XMLSchema#"
         xmlns:rdfs="http://www.w3.org/2000/01/rdf-schema#"
         xmlns:owl="http://www.w3.org/2002/07/owl#"
         xml:base="http://rukmal.me/precis"
         xmlns="http://rukmal.me/precis#"
         xmlns:x_1.1="http://purl.org/dc/elements/1.1/">

<owl:Ontology rdf:about="http://rukmal.me/precis">
  <owl:versionIRI rdf:resource="http://rukmal.me/precis/1.2.0"/>
  <x_1.1:creator rdf:resource="https://orcid.org/0000-0002-8628-6753"/>
  <rdfs:comment rdf:datatype="http://www.w3.org/2001/XMLSchema#string">The Precis ontology is designed to encapsulate portfolio information about an individual. This includes information that would traditionally be presented in a Resume/CV. This ontology is designed to be used with the Precis toolkit; see http://github.com/rukmal/precis for more.</rdfs:comment>
  <owl:versionInfo rdf:datatype="http://www.w3.org/2001/XMLSchema#string">1.2.0</owl:versionInfo>
</owl:Ontology>

<owl:AnnotationProperty rdf:about="http://purl.org/dc/elements/1.1/creator"/>

<rdfs:Datatype rdf:about="http://www.w3.org/2001/XMLSchema#gMonth"/>

<rdfs:Datatype rdf:about="http://www.w3.org/2001/XMLSchema#gYear"/>

<owl:ObjectProperty rdf:about="#affiliatedWith">
  <rdfs:domain>
    <owl:Class>
      <owl:unionOf rdf:parseType="Collection">
        <rdf:Description rdf:about="#Accolade"/>
        <rdf:Description rdf:about="#Portfolio"/>
      </owl:unionOf>
    </owl:Class>
  </rdfs:domain>
  <rdfs:range>
    <owl:Class>
      <owl:unionOf rdf:parseType="Collection">
        <rdf:Description rdf:about="#Degree"/>
        <rdf:Description rdf:about="#WorkExperience"/>
      </owl:unionOf>
    </owl:Class>
  </rdfs:range>
  <owl:inverseOf rdf:resource="#hasObject"/>
  <rdfs:comment>Affiliation for a Portfolio Instance or Accolade Instance. Maps a given instance to an instance of 'Degree' or 'WorkExperience'.</rdfs:comment>
  <rdfs:label>Affiliation</rdfs:label>
</owl:ObjectProperty>

<owl:ObjectProperty rdf:about="#hasObject">
  <rdf:type rdf:resource="http://www.w3.org/2002/07/owl#InverseFunctionalProperty"/>
  <rdfs:domain>
    <owl:Class>
      <owl:unionOf rdf:parseType="Collection">
        <rdf:Description rdf:about="#Degree"/>
        <rdf:Description rdf:about="#WorkExperience"/>
      </owl:unionOf>
    </owl:Class>
  </rdfs:domain>
  <rdfs:range>
    <owl:Class>
      <owl:unionOf rdf:parseType="Collection">
        <rdf:Description rdf:about="#Accolade"/>
        <rdf:Description rdf:about="#Portfolio"/>
      </owl:unionOf>
    </owl:Class>
  </rdfs:range>
  <rdfs:comment>Object that was affiliated with the Thing pointing to it. Here, "Object" would be typically a 'Portfolio' or 'Accolade' instance, and "Thing" would be a 'Degree' or 'WorkExperience' instance.</rdfs:comment>
  <rdfs:label>Constituent Object</rdfs:label>
</owl:ObjectProperty>

<owl:Class rdf:about="#Accolade">
  <rdfs:subClassOf>
    <owl:Restriction>
      <owl:onProperty rdf:resource="#affiliatedWith"/>
      <owl:someValuesFrom>
        <owl:Class>
          <owl:unionOf rdf:parseType="Collection">
            <rdf:Description rdf:about="#Degree"/>
            <rdf:Description rdf:about="#WorkExperience"/>
          </owl:unionOf>
        </owl:Class>
      </owl:someValuesFrom>
    </owl:Restriction>
  </rdfs:subClassOf>
  <rdfs:subClassOf>
    <owl:Restriction>
      <owl:onProperty rdf:resource="#hasDescription"/>
      <owl:onClass rdf:resource="#Description"/>
      <owl:minQualifiedCardinality rdf:datatype="http://www.w3.org/2001/XMLSchema#nonNegativeInteger">1</owl:minQualifiedCardinality>
    </owl:Restriction>
  </rdfs:subClassOf>
  <rdfs:subClassOf>
    <owl:Restriction>
      <owl:onProperty rdf:resource="#externalResource"/>
      <owl:someValuesFrom rdf:resource="http://www.w3.org/2001/XMLSchema#anyURI"/>
    </owl:Restriction>
  </rdfs:subClassOf>
  <rdfs:subClassOf>
    <owl:Restriction>
      <owl:onProperty rdf:resource="#hasMedia"/>
      <owl:someValuesFrom rdf:resource="http://www.w3.org/2001/XMLSchema#anyURI"/>
    </owl:Restriction>
  </rdfs:subClassOf>
  <rdfs:subClassOf>
    <owl:Restriction>
      <owl:onProperty rdf:resource="#hasDate"/>
      <owl:onDataRange rdf:resource="http://www.w3.org/2001/XMLSchema#dateTime"/>
      <owl:minQualifiedCardinality rdf:datatype="http://www.w3.org/2001/XMLSchema#nonNegativeInteger">1</owl:minQualifiedCardinality>
    </owl:Restriction>
  </rdfs:subClassOf>
  <rdfs:subClassOf>
    <owl:Restriction>
      <owl:onProperty rdf:resource="#hasName"/>
      <owl:onDataRange rdf:resource="http://www.w3.org/2001/XMLSchema#string"/>
      <owl:minQualifiedCardinality rdf:datatype="http://www.w3.org/2001/XMLSchema#nonNegativeInteger">1</owl:minQualifiedCardinality>
    </owl:Restriction>
  </rdfs:subClassOf>
  <rdfs:comment>An accolade. This is either an 'Award' or a 'Certification'.</rdfs:comment>
  <rdfs:label>Accolade</rdfs:label>
</owl:Class>

<owl:Class rdf:about="#Portfolio">
  <rdfs:subClassOf>
    <owl:Restriction>
      <owl:onProperty rdf:resource="#affiliatedWith"/>
      <owl:someValuesFrom>
        <owl:Class>
          <owl:unionOf rdf:parseType="Collection">
            <rdf:Description rdf:about="#Degree"/>
            <rdf:Description rdf:about="#WorkExperience"/>
          </owl:unionOf>
        </owl:Class>
      </owl:someValuesFrom>
    </owl:Restriction>
  </rdfs:subClassOf>
  <rdfs:subClassOf>
    <owl:Restriction>
      <owl:onProperty rdf:resource="#hasDescription"/>
      <owl:onClass rdf:resource="#Description"/>
      <owl:minQualifiedCardinality rdf:datatype="http://www.w3.org/2001/XMLSchema#nonNegativeInteger">1</owl:minQualifiedCardinality>
    </owl:Restriction>
  </rdfs:subClassOf>
  <rdfs:subClassOf>
    <owl:Restriction>
      <owl:onProperty rdf:resource="#endDate"/>
      <owl:someValuesFrom rdf:resource="http://www.w3.org/2001/XMLSchema#dateTime"/>
    </owl:Restriction>
  </rdfs:subClassOf>
  <rdfs:subClassOf>
    <owl:Restriction>
      <owl:onProperty rdf:resource="#externalResource"/>
      <owl:someValuesFrom rdf:resource="http://www.w3.org/2001/XMLSchema#anyURI"/>
    </owl:Restriction>
  </rdfs:subClassOf>
  <rdfs:subClassOf>
    <owl:Restriction>
      <owl:onProperty rdf:resource="#hasMedia"/>
      <owl:someValuesFrom rdf:resource="http://www.w3.org/2001/XMLSchema#anyURI"/>
    </owl:Restriction>
  </rdfs:subClassOf>
  <rdfs:subClassOf>
    <owl:Restriction>
      <owl:onProperty rdf:resource="#hasDate"/>
      <owl:onDataRange rdf:resource="http://www.w3.org/2001/XMLSchema#dateTime"/>
      <owl:minQualifiedCardinality rdf:datatype="http://www.w3.org/2001/XMLSchema#nonNegativeInteger">1</owl:minQualifiedCardinality>
    </owl:Restriction>
  </rdfs:subClassOf>
  <rdfs:subClassOf>
    <owl:Restriction>
      <owl:onProperty rdf:resource="#hasWebsite"/>
      <owl:onDataRange rdf:resource="http://www.w3.org/2001/XMLSchema#anyURI"/>
      <owl:minQualifiedCardinality rdf:datatype="http://www.w3.org/2001/XMLSchema#nonNegativeInteger">1</owl:minQualifiedCardinality>
    </owl:Restriction>
  </rdfs:subClassOf>
  <rdfs:subClassOf>
    <owl:Restriction>
      <owl:onProperty rdf:resource="#hasName"/>
      <owl:onDataRange rdf:resource="http://www.w3.org/2001/XMLSchema#string"/>
      <owl:qualifiedCardinality rdf:datatype="http://www.w3.org/2001/XMLSchema#nonNegativeInteger">1</owl:qualifiedCardinality>
    </owl:Restriction>
  </rdfs:subClassOf>
  <rdfs:comment>A Portfolio item; this can be a Talk, Publication, Project, etc.</rdfs:comment>
  <rdfs:label>Portfolio</rdfs:label>
</owl:Class>

<owl:Class rdf:about="#Degree">
  <rdfs:subClassOf>
    <owl:Restriction>
      <owl:onProperty rdf:resource="#degreeDepartment"/>
      <owl:someValuesFrom rdf:resource="#Organization"/>
    </owl:Restriction>
  </rdfs:subClassOf>
  <rdfs:subClassOf>
    <owl:Restriction>
      <owl:onProperty rdf:resource="#degreeSchool"/>
      <owl:someValuesFrom rdf:resource="#Organization"/>
    </owl:Restriction>
  </rdfs:subClassOf>
  <rdfs:subClassOf>
    <owl:Restriction>
      <owl:onProperty rdf:resource="#degreeUniversity"/>
      <owl:onClass rdf:resource="#Organization"/>
      <owl:minQualifiedCardinality rdf:datatype="http://www.w3.org/2001/XMLSchema#nonNegativeInteger">1</owl:minQualifiedCardinality>
    </owl:Restriction>
  </rdfs:subClassOf>
  <rdfs:subClassOf>
    <owl:Restriction>
      <owl:onProperty rdf:resource="#degreeConcentration"/>
      <owl:someValuesFrom rdf:resource="http://www.w3.org/2001/XMLSchema#anyURI"/>
    </owl:Restriction>
  </rdfs:subClassOf>
  <rdfs:subClassOf>
    <owl:Restriction>
      <owl:onProperty rdf:resource="#degreeGPA"/>
      <owl:someValuesFrom rdf:resource="http://www.w3.org/2001/XMLSchema#double"/>
    </owl:Restriction>
  </rdfs:subClassOf>
  <rdfs:subClassOf>
    <owl:Restriction>
      <owl:onProperty rdf:resource="#degreeType"/>
      <owl:someValuesFrom rdf:resource="http://www.w3.org/2001/XMLSchema#anyURI"/>
    </owl:Restriction>
  </rdfs:subClassOf>
  <rdfs:subClassOf>
    <owl:Restriction>
      <owl:onProperty rdf:resource="#hasDate"/>
      <owl:onDataRange rdf:resource="http://www.w3.org/2001/XMLSchema#dateTime"/>
      <owl:qualifiedCardinality rdf:datatype="http://www.w3.org/2001/XMLSchema#nonNegativeInteger">1</owl:qualifiedCardinality>
    </owl:Restriction>
  </rdfs:subClassOf>
  <rdfs:subClassOf>
    <owl:Restriction>
      <owl:onProperty rdf:resource="#hasName"/>
      <owl:onDataRange rdf:resource="http://www.w3.org/2001/XMLSchema#string"/>
      <owl:qualifiedCardinality rdf:datatype="http://www.w3.org/2001/XMLSchema#nonNegativeInteger">1</owl:qualifiedCardinality>
    </owl:Restriction>
  </rdfs:subClassOf>
  <rdfs:subClassOf>
    <owl:Restriction>
      <owl:onProperty rdf:resource="#inCity"/>
      <owl:onDataRange rdf:resource="http://www.w3.org/2001/XMLSchema#string"/>
      <owl:qualifiedCardinality rdf:datatype="http://www.w3.org/2001/XMLSchema#nonNegativeInteger">1</owl:qualifiedCardinality>
    </owl:Restriction>
  </rdfs:subClassOf>
  <rdfs:subClassOf>
    <owl:Restriction>
      <owl:onProperty rdf:resource="#inState"/>
      <owl:onDataRange rdf:resource="http://www.w3.org/2001/XMLSchema#string"/>
      <owl:qualifiedCardinality rdf:datatype="http://www.w3.org/2001/XMLSchema#nonNegativeInteger">1</owl:qualifiedCardinality>
    </owl:Restriction>
  </rdfs:subClassOf>
  <rdfs:comment>A Degree, which was completed at a specific institution, in a specific school and department. Optional media links to pictures can be included for rendering at the time of presentation. Records the year and month that the degree was (or is expected to be) awarded.</rdfs:comment>
  <rdfs:label>Degree</rdfs:label>
</owl:Class>

<owl:Class rdf:about="#WorkExperience">
  <rdfs:subClassOf>
    <owl:Class>
      <owl:unionOf rdf:parseType="Collection">
        <owl:Restriction>
          <owl:onProperty rdf:resource="#inCountry"/>
          <owl:onDataRange rdf:resource="http://www.w3.org/2001/XMLSchema#string"/>
          <owl:qualifiedCardinality rdf:datatype="http://www.w3.org/2001/XMLSchema#nonNegativeInteger">1</owl:qualifiedCardinality>
        </owl:Restriction>
        <owl:Restriction>
          <owl:onProperty rdf:resource="#inState"/>
          <owl:onDataRange rdf:resource="http://www.w3.org/2001/XMLSchema#string"/>
          <owl:qualifiedCardinality rdf:datatype="http://www.w3.org/2001/XMLSchema#nonNegativeInteger">1</owl:qualifiedCardinality>
        </owl:Restriction>
      </owl:unionOf>
    </owl:Class>
  </rdfs:subClassOf>
  <rdfs:subClassOf>
    <owl:Restriction>
      <owl:onProperty rdf:resource="#hasDescription"/>
      <owl:onClass rdf:resource="#Description"/>
      <owl:minQualifiedCardinality rdf:datatype="http://www.w3.org/2001/XMLSchema#nonNegativeInteger">1</owl:minQualifiedCardinality>
    </owl:Restriction>
  </rdfs:subClassOf>
  <rdfs:subClassOf>
    <owl:Restriction>
      <owl:onProperty rdf:resource="#employedAt"/>
      <owl:onClass rdf:resource="#Organization"/>
      <owl:qualifiedCardinality rdf:datatype="http://www.w3.org/2001/XMLSchema#nonNegativeInteger">1</owl:qualifiedCardinality>
    </owl:Restriction>
  </rdfs:subClassOf>
  <rdfs:subClassOf>
    <owl:Restriction>
      <owl:onProperty rdf:resource="#endDate"/>
      <owl:someValuesFrom rdf:resource="http://www.w3.org/2001/XMLSchema#dateTime"/>
    </owl:Restriction>
  </rdfs:subClassOf>
  <rdfs:subClassOf>
    <owl:Restriction>
      <owl:onProperty rdf:resource="#hasImage"/>
      <owl:someValuesFrom rdf:resource="http://www.w3.org/2001/XMLSchema#anyURI"/>
    </owl:Restriction>
  </rdfs:subClassOf>
  <rdfs:subClassOf>
    <owl:Restriction>
      <owl:onProperty rdf:resource="#hasMedia"/>
      <owl:someValuesFrom rdf:resource="http://www.w3.org/2001/XMLSchema#anyURI"/>
    </owl:Restriction>
  </rdfs:subClassOf>
  <rdfs:subClassOf>
    <owl:Restriction>
      <owl:onProperty rdf:resource="#hasDate"/>
      <owl:onDataRange rdf:resource="http://www.w3.org/2001/XMLSchema#dateTime"/>
      <owl:minQualifiedCardinality rdf:datatype="http://www.w3.org/2001/XMLSchema#nonNegativeInteger">1</owl:minQualifiedCardinality>
    </owl:Restriction>
  </rdfs:subClassOf>
  <rdfs:subClassOf>
    <owl:Restriction>
      <owl:onProperty rdf:resource="#jobTitle"/>
      <owl:onDataRange rdf:resource="http://www.w3.org/2001/XMLSchema#string"/>
      <owl:minQualifiedCardinality rdf:datatype="http://www.w3.org/2001/XMLSchema#nonNegativeInteger">1</owl:minQualifiedCardinality>
    </owl:Restriction>
  </rdfs:subClassOf>
  <rdfs:subClassOf>
    <owl:Restriction>
      <owl:onProperty rdf:resource="#inCity"/>
      <owl:onDataRange rdf:resource="http://www.w3.org/2001/XMLSchema#string"/>
      <owl:qualifiedCardinality rdf:datatype="http://www.w3.org/2001/XMLSchema#nonNegativeInteger">1</owl:qualifiedCardinality>
    </owl:Restriction>
  </rdfs:subClassOf>
  <rdfs:comment>An instance of 'Work Experience'. This would be an internship/assistantship/etc.</rdfs:comment>
  <rdfs:label>Work Experience</rdfs:label>
</owl:Class>

<owl:ObjectProperty rdf:about="#awardedDegree">
  <rdf:type rdf:resource="http://www.w3.org/2002/07/owl#InverseFunctionalProperty"/>
  <rdfs:domain rdf:resource="#Organization"/>
  <rdfs:range rdf:resource="#Degree"/>
  <owl:inverseOf rdf:resource="#degreeUniversity"/>
  <rdfs:comment>The Degree which was awarded at this organization (should be a pointer to a top-level organization).</rdfs:comment>
  <rdfs:label>Degree awarded</rdfs:label>
</owl:ObjectProperty>

<owl:ObjectProperty rdf:about="#degreeUniversity">
  <rdfs:domain rdf:resource="#Degree"/>
  <rdfs:range rdf:resource="#Organization"/>
  <rdfs:comment>The University (concept: Organization) at which the degree was awarded. This corresponds to the top-level instituion; further object properties exist to specify particular schools/departments. That is, this should point to the organization for the Univesity and not the Department. Eg: awardedAt 'University of Washington'; and should NOT be awardedAt 'Foster School of Business'.</rdfs:comment>
  <rdfs:label>Organization awarding the Degree</rdfs:label>
</owl:ObjectProperty>

<owl:Class rdf:about="#Organization">
  <rdfs:subClassOf>
    <owl:Restriction>
      <owl:onProperty rdf:resource="#hasParentOrganization"/>
      <owl:someValuesFrom rdf:resource="#Organization"/>
    </owl:Restriction>
  </rdfs:subClassOf>
  <rdfs:subClassOf>
    <owl:Restriction>
      <owl:onProperty rdf:resource="#hasDescription"/>
      <owl:onClass rdf:resource="#Description"/>
      <owl:maxQualifiedCardinality rdf:datatype="http://www.w3.org/2001/XMLSchema#nonNegativeInteger">1</owl:maxQualifiedCardinality>
    </owl:Restriction>
  </rdfs:subClassOf>
  <rdfs:subClassOf>
    <owl:Restriction>
      <owl:onProperty rdf:resource="#externalResource"/>
      <owl:someValuesFrom rdf:resource="http://www.w3.org/2001/XMLSchema#anyURI"/>
    </owl:Restriction>
  </rdfs:subClassOf>
  <rdfs:subClassOf>
    <owl:Restriction>
      <owl:onProperty rdf:resource="#hasName"/>
      <owl:onDataRange rdf:resource="http://www.w3.org/2001/XMLSchema#string"/>
      <owl:qualifiedCardinality rdf:datatype="http://www.w3.org/2001/XMLSchema#nonNegativeInteger">1</owl:qualifiedCardinality>
    </owl:Restriction>
  </rdfs:subClassOf>
  <rdfs:subClassOf>
    <owl:Restriction>
      <owl:onProperty rdf:resource="#hasWebsite"/>
      <owl:onDataRange rdf:resource="http://www.w3.org/2001/XMLSchema#anyURI"/>
      <owl:qualifiedCardinality rdf:datatype="http://www.w3.org/2001/XMLSchema#nonNegativeInteger">1</owl:qualifiedCardinality>
    </owl:Restriction>
  </rdfs:subClassOf>
  <rdfs:comment>An organization; this can be a company, university, a specific university department, etc.</rdfs:comment>
  <rdfs:label>Organization</rdfs:label>
</owl:Class>

<owl:ObjectProperty rdf:about="#degreeDepartment">
  <rdfs:domain rdf:resource="#Degree"/>
  <rdfs:range rdf:resource="#Organization"/>
  <rdfs:comment>Department awarding the degree (eg: "Department of Financial Engineering", or "Department of Finance and Business Economics").</rdfs:comment>
  <rdfs:label>Department awarding the Degree</rdfs:label>
</owl:ObjectProperty>

<owl:ObjectProperty rdf:about="#degreeSchool">
  <rdfs:domain rdf:resource="#Degree"/>
  <rdfs:range rdf:resource="#Organization"/>
  <rdfs:comment>The School that awards the degree. For example, this would be the "Foster School of Business", or "College of Arts and Sciences".</rdfs:comment>
  <rdfs:label>School awarding the Degree</rdfs:label>
</owl:ObjectProperty>

<owl:ObjectProperty rdf:about="#employedAt">
  <rdf:type rdf:resource="http://www.w3.org/2002/07/owl#InverseFunctionalProperty"/>
  <rdfs:domain rdf:resource="#WorkExperience"/>
  <rdfs:range rdf:resource="#Organization"/>
  <rdfs:comment>Organization where an instance of Work Experience is taking place.</rdfs:comment>
  <rdfs:label>Employment Organization</rdfs:label>
</owl:ObjectProperty>

<owl:ObjectProperty rdf:about="#hasChildOrganization">
  <rdf:type rdf:resource="http://www.w3.org/2002/07/owl#TransitiveProperty"/>
  <rdfs:domain rdf:resource="#Organization"/>
  <rdfs:range rdf:resource="#Organization"/>
  <owl:inverseOf rdf:resource="#hasParentOrganization"/>
  <rdfs:comment>Child organization pointer, inverse of the 'hasParentOrganization' property.</rdfs:comment>
  <rdfs:label>Child Organization</rdfs:label>
</owl:ObjectProperty>

<owl:ObjectProperty rdf:about="#hasParentOrganization">
  <rdf:type rdf:resource="http://www.w3.org/2002/07/owl#TransitiveProperty"/>
  <rdfs:domain rdf:resource="#Organization"/>
  <rdfs:range rdf:resource="#Organization"/>
  <rdfs:comment>Pointer to a "parent" organization instance. For example, the "Foster School of Business" hasParentOrganization "University of Washington".</rdfs:comment>
  <rdfs:label>Parent Organization</rdfs:label>
</owl:ObjectProperty>

<owl:ObjectProperty rdf:about="#hasDescription">
  <rdfs:domain>
    <owl:Class>
      <owl:unionOf rdf:parseType="Collection">
        <rdf:Description rdf:about="#Accolade"/>
        <rdf:Description rdf:about="#ActivityType"/>
        <rdf:Description rdf:about="#Course"/>
        <rdf:Description rdf:about="#KnowledgeArea"/>
        <rdf:Description rdf:about="#Organization"/>
        <rdf:Description rdf:about="#Portfolio"/>
        <rdf:Description rdf:about="#SkillGroup"/>
        <rdf:Description rdf:about="#WorkExperience"/>
      </owl:unionOf>
    </owl:Class>
  </rdfs:domain>
  <rdfs:range rdf:resource="#Description"/>
  <rdfs:comment>Instance of 'Description', which describes the Thing pointing to it.</rdfs:comment>
  <rdfs:label>Description</rdfs:label>
</owl:ObjectProperty>

<owl:Class rdf:about="#ActivityType">
  <rdfs:subClassOf>
    <owl:Restriction>
      <owl:onProperty rdf:resource="#hasDescription"/>
      <owl:onClass rdf:resource="#Description"/>
      <owl:minQualifiedCardinality rdf:datatype="http://www.w3.org/2001/XMLSchema#nonNegativeInteger">1</owl:minQualifiedCardinality>
    </owl:Restriction>
  </rdfs:subClassOf>
  <rdfs:subClassOf>
    <owl:Restriction>
      <owl:onProperty rdf:resource="#endDate"/>
      <owl:someValuesFrom rdf:resource="http://www.w3.org/2001/XMLSchema#dateTime"/>
    </owl:Restriction>
  </rdfs:subClassOf>
  <rdfs:subClassOf>
    <owl:Restriction>
      <owl:onProperty rdf:resource="#externalResource"/>
      <owl:someValuesFrom rdf:resource="http://www.w3.org/2001/XMLSchema#anyURI"/>
    </owl:Restriction>
  </rdfs:subClassOf>
  <rdfs:subClassOf>
    <owl:Restriction>
      <owl:onProperty rdf:resource="#hasDate"/>
      <owl:someValuesFrom rdf:resource="http://www.w3.org/2001/XMLSchema#dateTime"/>
    </owl:Restriction>
  </rdfs:subClassOf>
  <rdfs:subClassOf>
    <owl:Restriction>
      <owl:onProperty rdf:resource="#hasMedia"/>
      <owl:someValuesFrom rdf:resource="http://www.w3.org/2001/XMLSchema#anyURI"/>
    </owl:Restriction>
  </rdfs:subClassOf>
  <rdfs:subClassOf>
    <owl:Restriction>
      <owl:onProperty rdf:resource="#hasName"/>
      <owl:onDataRange rdf:resource="http://www.w3.org/2001/XMLSchema#string"/>
      <owl:minQualifiedCardinality rdf:datatype="http://www.w3.org/2001/XMLSchema#nonNegativeInteger">1</owl:minQualifiedCardinality>
    </owl:Restriction>
  </rdfs:subClassOf>
  <rdfs:comment>Type of the activity (typically a larger supergroup), such as "Hackathon" or "Volunteering".</rdfs:comment>
  <rdfs:label>Activity Type</rdfs:label>
</owl:Class>

<owl:Class rdf:about="#Course">
  <rdfs:subClassOf>
    <owl:Restriction>
      <owl:onProperty rdf:resource="#hasDescription"/>
      <owl:someValuesFrom rdf:resource="#Description"/>
    </owl:Restriction>
  </rdfs:subClassOf>
  <rdfs:subClassOf>
    <owl:Restriction>
      <owl:onProperty rdf:resource="#taughtAt"/>
      <owl:someValuesFrom rdf:resource="#Organization"/>
    </owl:Restriction>
  </rdfs:subClassOf>
  <rdfs:subClassOf>
    <owl:Restriction>
      <owl:onProperty rdf:resource="#endDate"/>
      <owl:someValuesFrom rdf:resource="http://www.w3.org/2001/XMLSchema#dateTime"/>
    </owl:Restriction>
  </rdfs:subClassOf>
  <rdfs:subClassOf>
    <owl:Restriction>
      <owl:onProperty rdf:resource="#hasCourseCode"/>
      <owl:someValuesFrom rdf:resource="http://www.w3.org/2001/XMLSchema#string"/>
    </owl:Restriction>
  </rdfs:subClassOf>
  <rdfs:subClassOf>
    <owl:Restriction>
      <owl:onProperty rdf:resource="#hasDate"/>
      <owl:someValuesFrom rdf:resource="http://www.w3.org/2001/XMLSchema#dateTime"/>
    </owl:Restriction>
  </rdfs:subClassOf>
  <rdfs:subClassOf>
    <owl:Restriction>
      <owl:onProperty rdf:resource="#hasDepartmentCode"/>
      <owl:someValuesFrom rdf:resource="http://www.w3.org/2001/XMLSchema#string"/>
    </owl:Restriction>
  </rdfs:subClassOf>
  <rdfs:subClassOf>
    <owl:Restriction>
      <owl:onProperty rdf:resource="#withGrade"/>
      <owl:someValuesFrom rdf:resource="http://www.w3.org/2001/XMLSchema#double"/>
    </owl:Restriction>
  </rdfs:subClassOf>
  <rdfs:subClassOf>
    <owl:Restriction>
      <owl:onProperty rdf:resource="#hasName"/>
      <owl:onDataRange rdf:resource="http://www.w3.org/2001/XMLSchema#string"/>
      <owl:qualifiedCardinality rdf:datatype="http://www.w3.org/2001/XMLSchema#nonNegativeInteger">1</owl:qualifiedCardinality>
    </owl:Restriction>
  </rdfs:subClassOf>
  <rdfs:subClassOf>
    <owl:Restriction>
      <owl:onProperty rdf:resource="#hasWebsite"/>
      <owl:onDataRange rdf:resource="http://www.w3.org/2001/XMLSchema#anyURI"/>
      <owl:qualifiedCardinality rdf:datatype="http://www.w3.org/2001/XMLSchema#nonNegativeInteger">1</owl:qualifiedCardinality>
    </owl:Restriction>
  </rdfs:subClassOf>
  <rdfs:comment>A course. This would typically be an item that is included in the "Relevant Coursework" section of a Resume/CV.</rdfs:comment>
  <rdfs:label>Course</rdfs:label>
</owl:Class>

<owl:Class rdf:about="#KnowledgeArea">
  <rdfs:subClassOf>
    <owl:Restriction>
      <owl:onProperty rdf:resource="#hasDescription"/>
      <owl:onClass rdf:resource="#Description"/>
      <owl:minQualifiedCardinality rdf:datatype="http://www.w3.org/2001/XMLSchema#nonNegativeInteger">1</owl:minQualifiedCardinality>
    </owl:Restriction>
  </rdfs:subClassOf>
  <rdfs:subClassOf>
    <owl:Restriction>
      <owl:onProperty rdf:resource="#externalResource"/>
      <owl:onDataRange rdf:resource="http://www.w3.org/2001/XMLSchema#anyURI"/>
      <owl:minQualifiedCardinality rdf:datatype="http://www.w3.org/2001/XMLSchema#nonNegativeInteger">1</owl:minQualifiedCardinality>
    </owl:Restriction>
  </rdfs:subClassOf>
  <rdfs:subClassOf>
    <owl:Restriction>
      <owl:onProperty rdf:resource="#hasName"/>
      <owl:onDataRange rdf:resource="http://www.w3.org/2001/XMLSchema#string"/>
      <owl:minQualifiedCardinality rdf:datatype="http://www.w3.org/2001/XMLSchema#nonNegativeInteger">1</owl:minQualifiedCardinality>
    </owl:Restriction>
  </rdfs:subClassOf>
  <rdfs:comment>Knowledge Area parent group. This would be something along the lines of "Mathematics", or "Computer Science".</rdfs:comment>
  <rdfs:label>Knowledge Area</rdfs:label>
</owl:Class>

<owl:Class rdf:about="#SkillGroup">
  <rdfs:subClassOf>
    <owl:Restriction>
      <owl:onProperty rdf:resource="#hasDescription"/>
      <owl:someValuesFrom rdf:resource="#Description"/>
    </owl:Restriction>
  </rdfs:subClassOf>
  <rdfs:subClassOf>
    <owl:Restriction>
      <owl:onProperty rdf:resource="#externalResource"/>
      <owl:someValuesFrom rdf:resource="http://www.w3.org/2001/XMLSchema#anyURI"/>
    </owl:Restriction>
  </rdfs:subClassOf>
  <rdfs:subClassOf>
    <owl:Restriction>
      <owl:onProperty rdf:resource="#hasName"/>
      <owl:onDataRange rdf:resource="http://www.w3.org/2001/XMLSchema#string"/>
      <owl:qualifiedCardinality rdf:datatype="http://www.w3.org/2001/XMLSchema#nonNegativeInteger">1</owl:qualifiedCardinality>
    </owl:Restriction>
  </rdfs:subClassOf>
  <rdfs:comment>A Skill Group. This group can contain one or more Skills. For example, "Python", "R", and "Java" would all be in the "Programming Languages" Skill Group.</rdfs:comment>
  <rdfs:label>Skill Group</rdfs:label>
</owl:Class>

<owl:Class rdf:about="#Description">
  <rdfs:subClassOf>
    <owl:Restriction>
      <owl:onProperty rdf:resource="#hasText"/>
      <owl:onDataRange rdf:resource="http://www.w3.org/2001/XMLSchema#string"/>
      <owl:qualifiedCardinality rdf:datatype="http://www.w3.org/2001/XMLSchema#nonNegativeInteger">1</owl:qualifiedCardinality>
    </owl:Restriction>
  </rdfs:subClassOf>
  <rdfs:subClassOf>
    <owl:Restriction>
      <owl:onProperty rdf:resource="#hasPriority"/>
      <owl:onDataRange rdf:resource="http://www.w3.org/2001/XMLSchema#nonNegativeInteger"/>
      <owl:maxQualifiedCardinality rdf:datatype="http://www.w3.org/2001/XMLSchema#nonNegativeInteger">1</owl:maxQualifiedCardinality>
    </owl:Restriction>
  </rdfs:subClassOf>
  <rdfs:comment>This description is associated with any other concept, providing a description. It has the capability to track priority levels, which can be used to intelligently truncate a series of descriptions when creating a Resume/CV with the command line toolkit.</rdfs:comment>
  <rdfs:label>Description for a given item</rdfs:label>
</owl:Class>

<owl:ObjectProperty rdf:about="#hasSubject">
  <rdf:type rdf:resource="http://www.w3.org/2002/07/owl#InverseFunctionalProperty"/>
  <rdfs:domain rdf:resource="#KnowledgeArea"/>
  <rdfs:range rdf:resource="#Subject"/>
  <owl:inverseOf rdf:resource="#inKnowledgeArea"/>
  <rdfs:comment>A subject that is a part of a 'KnowledgeArea'.</rdfs:comment>
  <rdfs:label>Constituent Subject</rdfs:label>
</owl:ObjectProperty>

<owl:ObjectProperty rdf:about="#inKnowledgeArea">
  <rdfs:domain rdf:resource="#Subject"/>
  <rdfs:range rdf:resource="#KnowledgeArea"/>
  <rdfs:comment>The knowledge area containing the subject.</rdfs:comment>
  <rdfs:label>Parent Knowledge Area</rdfs:label>
</owl:ObjectProperty>

<owl:Class rdf:about="#Subject">
  <rdfs:subClassOf rdf:resource="#KnowledgeArea"/>
  <rdfs:subClassOf>
    <owl:Restriction>
      <owl:onProperty rdf:resource="#hasName"/>
      <owl:onDataRange rdf:resource="http://www.w3.org/2001/XMLSchema#string"/>
      <owl:minQualifiedCardinality rdf:datatype="http://www.w3.org/2001/XMLSchema#nonNegativeInteger">1</owl:minQualifiedCardinality>
    </owl:Restriction>
  </rdfs:subClassOf>
  <rdfs:comment>Specific subject in a Knowledge Area. This would be "Distributed Systems" in the Knowledge Area of "Mathematics", or "Real Analysis" in the "Mathematics" Knowledge Area.</rdfs:comment>
  <rdfs:label>Specific Subject</rdfs:label>
</owl:Class>

<owl:ObjectProperty rdf:about="#relatedTo">
  <rdf:type rdf:resource="http://www.w3.org/2002/07/owl#SymmetricProperty"/>
  <rdf:type rdf:resource="http://www.w3.org/2002/07/owl#TransitiveProperty"/>
  <rdfs:domain>
    <owl:Class>
      <owl:unionOf rdf:parseType="Collection">
        <rdf:Description rdf:about="#Accolade"/>
        <rdf:Description rdf:about="#Activity"/>
        <rdf:Description rdf:about="#Course"/>
        <rdf:Description rdf:about="#Degree"/>
        <rdf:Description rdf:about="#Portfolio"/>
        <rdf:Description rdf:about="#Skill"/>
        <rdf:Description rdf:about="#Subject"/>
        <rdf:Description rdf:about="#WorkExperience"/>
      </owl:unionOf>
    </owl:Class>
  </rdfs:domain>
  <rdfs:range>
    <owl:Class>
      <owl:unionOf rdf:parseType="Collection">
        <rdf:Description rdf:about="#Accolade"/>
        <rdf:Description rdf:about="#Activity"/>
        <rdf:Description rdf:about="#Course"/>
        <rdf:Description rdf:about="#Degree"/>
        <rdf:Description rdf:about="#Portfolio"/>
        <rdf:Description rdf:about="#Skill"/>
        <rdf:Description rdf:about="#Subject"/>
        <rdf:Description rdf:about="#WorkExperience"/>
      </owl:unionOf>
    </owl:Class>
  </rdfs:range>
  <rdfs:comment>A related concept. For example, an instance of 'Award' may have a 'Project', or 'Publication' that it is related to, and vice versa.</rdfs:comment>
  <rdfs:label>Related Concept</rdfs:label>
</owl:ObjectProperty>

<owl:Class rdf:about="#Activity">
  <rdfs:subClassOf rdf:resource="#ActivityType"/>
  <rdfs:comment>A specific activity, such as a specific hackathon or volunteering experience.</rdfs:comment>
  <rdfs:label>Activity</rdfs:label>
</owl:Class>

<owl:Class rdf:about="#Skill">
  <rdfs:subClassOf rdf:resource="#SkillGroup"/>
  <rdfs:subClassOf>
    <owl:Restriction>
      <owl:onProperty rdf:resource="#externalResource"/>
      <owl:someValuesFrom rdf:resource="http://www.w3.org/2001/XMLSchema#anyURI"/>
    </owl:Restriction>
  </rdfs:subClassOf>
  <rdfs:subClassOf>
    <owl:Restriction>
      <owl:onProperty rdf:resource="#hasName"/>
      <owl:onDataRange rdf:resource="http://www.w3.org/2001/XMLSchema#string"/>
      <owl:qualifiedCardinality rdf:datatype="http://www.w3.org/2001/XMLSchema#nonNegativeInteger">1</owl:qualifiedCardinality>
    </owl:Restriction>
  </rdfs:subClassOf>
  <rdfs:comment>An individual skill. Each skill belongs to a specific SkillGroup. For example; "Python", "R", and "Java" would all be skills, in the "Programming Languages" SkillGroup.</rdfs:comment>
  <rdfs:label>Skill</rdfs:label>
</owl:Class>

<owl:ObjectProperty rdf:about="#taughtAt">
  <rdfs:domain rdf:resource="#Course"/>
  <rdfs:range rdf:resource="#Organization"/>
  <rdfs:comment>The organization at which the course was taught. This is an optional field, but ideally if this is included, the department and course codes should be too.</rdfs:comment>
  <rdfs:label>Organization which taught the course</rdfs:label>
</owl:ObjectProperty>

<owl:DatatypeProperty rdf:about="#degreeConcentration">
  <rdfs:domain rdf:resource="#Degree"/>
  <rdfs:range rdf:resource="http://www.w3.org/2001/XMLSchema#anyURI"/>
  <rdfs:comment>Concentration of the Degree. For example, "Finance and Business Economics", or "Computational Finance". This should point to a DBpedia entity corresponding to the Degree being awarded.</rdfs:comment>
  <rdfs:label>Degree Concentration</rdfs:label>
</owl:DatatypeProperty>

<owl:DatatypeProperty rdf:about="#degreeGPA">
  <rdfs:domain rdf:resource="#Degree"/>
  <rdfs:range>
    <rdfs:Datatype>
      <owl:onDatatype rdf:resource="http://www.w3.org/2001/XMLSchema#double"/>
      <owl:withRestrictions>
        <rdf:Description>
          <rdf:first>
            <rdf:Description>
              <xsd:minInclusive rdf:datatype="http://www.w3.org/2001/XMLSchema#double">0.0</xsd:minInclusive>
            </rdf:Description>
          </rdf:first>
          <rdf:rest>
            <rdf:Description>
              <rdf:first>
                <rdf:Description>
                  <xsd:maxInclusive rdf:datatype="http://www.w3.org/2001/XMLSchema#double">4.0</xsd:maxInclusive>
                </rdf:Description>
              </rdf:first>
              <rdf:rest rdf:resource="http://www.w3.org/1999/02/22-rdf-syntax-ns#nil"/>
            </rdf:Description>
          </rdf:rest>
        </rdf:Description>
      </owl:withRestrictions>
    </rdfs:Datatype>
  </rdfs:range>
  <rdfs:comment>Grade (GPA; 4.0 scale) for the Degree (optional for obvious reasons :)).</rdfs:comment>
  <rdfs:label>Degree GPA (on a 4.0 scale)</rdfs:label>
</owl:DatatypeProperty>

<owl:DatatypeProperty rdf:about="#degreeType">
  <rdfs:domain rdf:resource="#Degree"/>
  <rdfs:range rdf:resource="http://www.w3.org/2001/XMLSchema#anyURI"/>
  <rdfs:comment>Type of the Degree. For example, "Bachelor of Arts", or "Master of Science". This should point to a DBpedia entity corresponding to the Degree being awarded.</rdfs:comment>
  <rdfs:label>Degree Type</rdfs:label>
</owl:DatatypeProperty>

<owl:DatatypeProperty rdf:about="#endDate">
  <rdfs:domain>
    <owl:Class>
      <owl:unionOf rdf:parseType="Collection">
        <rdf:Description rdf:about="#ActivityType"/>
        <rdf:Description rdf:about="#Course"/>
        <rdf:Description rdf:about="#Portfolio"/>
        <rdf:Description rdf:about="#WorkExperience"/>
      </owl:unionOf>
    </owl:Class>
  </rdfs:domain>
  <rdfs:range rdf:resource="http://www.w3.org/2001/XMLSchema#dateTime"/>
  <rdfs:comment>End date of a Instance. When this is included, the 'hasDate' data property corresponds to the start date.</rdfs:comment>
  <rdfs:label>endDate</rdfs:label>
</owl:DatatypeProperty>

<owl:DatatypeProperty rdf:about="#externalResource">
  <rdfs:domain>
    <owl:Class>
      <owl:unionOf rdf:parseType="Collection">
        <rdf:Description rdf:about="#Accolade"/>
        <rdf:Description rdf:about="#ActivityType"/>
        <rdf:Description rdf:about="#Course"/>
        <rdf:Description rdf:about="#Degree"/>
        <rdf:Description rdf:about="#KnowledgeArea"/>
        <rdf:Description rdf:about="#Organization"/>
        <rdf:Description rdf:about="#Portfolio"/>
        <rdf:Description rdf:about="#SkillGroup"/>
        <rdf:Description rdf:about="#WorkExperience"/>
      </owl:unionOf>
    </owl:Class>
  </rdfs:domain>
  <rdfs:range rdf:resource="http://www.w3.org/2001/XMLSchema#anyURI"/>
  <rdfs:comment>Reference to an external resource that describes the same entity. This would typically be a reference to an existing DBpedia concept that describes the same entity. DBpedia references are not directly used here to mitigate the fact that certain user-created entitites will not have existing concepts on DBpedia, and so that we can ensure the existence of some other descriptive fields.</rdfs:comment>
  <rdfs:label>External resource</rdfs:label>
</owl:DatatypeProperty>

<owl:DatatypeProperty rdf:about="#hasAuthors">
  <rdfs:domain rdf:resource="#Publication"/>
  <rdfs:range rdf:resource="http://www.w3.org/2001/XMLSchema#string"/>
  <rdfs:comment>List of authors (Human readable for now). This list should mirror the order of authors in the publication. Note that eventually this will be replaced by pointers to individual "Author" Classes.</rdfs:comment>
  <rdfs:label>Author List</rdfs:label>
</owl:DatatypeProperty>

<owl:Class rdf:about="#Publication">
  <rdfs:subClassOf rdf:resource="#Portfolio"/>
  <rdfs:subClassOf>
    <owl:Restriction>
      <owl:onProperty rdf:resource="#hasAuthors"/>
      <owl:allValuesFrom rdf:resource="http://www.w3.org/2001/XMLSchema#string"/>
    </owl:Restriction>
  </rdfs:subClassOf>
  <rdfs:subClassOf>
    <owl:Restriction>
      <owl:onProperty rdf:resource="#hasDate"/>
      <owl:onDataRange rdf:resource="http://www.w3.org/2001/XMLSchema#dateTime"/>
      <owl:minQualifiedCardinality rdf:datatype="http://www.w3.org/2001/XMLSchema#nonNegativeInteger">1</owl:minQualifiedCardinality>
    </owl:Restriction>
  </rdfs:subClassOf>
  <rdfs:subClassOf>
    <owl:Restriction>
      <owl:onProperty rdf:resource="#inConferenceOrJournal"/>
      <owl:onDataRange rdf:resource="http://www.w3.org/2001/XMLSchema#string"/>
      <owl:qualifiedCardinality rdf:datatype="http://www.w3.org/2001/XMLSchema#nonNegativeInteger">1</owl:qualifiedCardinality>
    </owl:Restriction>
  </rdfs:subClassOf>
  <rdfs:subClassOf>
    <owl:Restriction>
      <owl:onProperty rdf:resource="#inPublication"/>
      <owl:onDataRange rdf:resource="http://www.w3.org/2001/XMLSchema#string"/>
      <owl:qualifiedCardinality rdf:datatype="http://www.w3.org/2001/XMLSchema#nonNegativeInteger">1</owl:qualifiedCardinality>
    </owl:Restriction>
  </rdfs:subClassOf>
  <rdfs:subClassOf>
    <owl:Restriction>
      <owl:onProperty rdf:resource="#hasDOI"/>
      <owl:onDataRange rdf:resource="http://www.w3.org/2001/XMLSchema#anyURI"/>
      <owl:maxQualifiedCardinality rdf:datatype="http://www.w3.org/2001/XMLSchema#nonNegativeInteger">1</owl:maxQualifiedCardinality>
    </owl:Restriction>
  </rdfs:subClassOf>
  <rdfs:subClassOf>
    <owl:Restriction>
      <owl:onProperty rdf:resource="#hasStatus"/>
      <owl:onDataRange rdf:resource="http://www.w3.org/2001/XMLSchema#string"/>
      <owl:maxQualifiedCardinality rdf:datatype="http://www.w3.org/2001/XMLSchema#nonNegativeInteger">1</owl:maxQualifiedCardinality>
    </owl:Restriction>
  </rdfs:subClassOf>
  <rdfs:comment>A publication, typically limited to peer reviewed articles.</rdfs:comment>
  <rdfs:label>Publication</rdfs:label>
</owl:Class>

<owl:DatatypeProperty rdf:about="#hasCollaborators">
  <rdfs:domain rdf:resource="#Portfolio"/>
  <rdfs:range rdf:resource="http://www.w3.org/2001/XMLSchema#string"/>
  <rdfs:comment>List of Collaborators (Human-readable for now). Will eventually change to a mapping to a Person entity.</rdfs:comment>
  <rdfs:label>Collaborators List</rdfs:label>
</owl:DatatypeProperty>

<owl:DatatypeProperty rdf:about="#hasCourseCode">
  <rdfs:domain rdf:resource="#Course"/>
  <rdfs:range rdf:resource="http://www.w3.org/2001/XMLSchema#string"/>
  <rdfs:comment>Code of the course (this would imply that an organization is referenced too). For example: 420, 690, 069, etc.</rdfs:comment>
  <rdfs:label>Course code</rdfs:label>
</owl:DatatypeProperty>

<owl:DatatypeProperty rdf:about="#hasDOI">
  <rdfs:domain rdf:resource="#Publication"/>
  <rdfs:range rdf:resource="http://www.w3.org/2001/XMLSchema#anyURI"/>
  <rdfs:comment>Digital Object Identifier (DOI) of the publication. Including this will allow for later expansion if an inference agent is ever added to get more metadata using this.</rdfs:comment>
  <rdfs:label>Digital Object Identifier (DOI) of the Publication</rdfs:label>
</owl:DatatypeProperty>

<owl:DatatypeProperty rdf:about="#hasDate">
  <rdfs:domain>
    <owl:Class>
      <owl:unionOf rdf:parseType="Collection">
        <rdf:Description rdf:about="#Accolade"/>
        <rdf:Description rdf:about="#ActivityType"/>
        <rdf:Description rdf:about="#Course"/>
        <rdf:Description rdf:about="#Degree"/>
        <rdf:Description rdf:about="#Portfolio"/>
        <rdf:Description rdf:about="#WorkExperience"/>
      </owl:unionOf>
    </owl:Class>
  </rdfs:domain>
  <rdfs:range rdf:resource="http://www.w3.org/2001/XMLSchema#dateTime"/>
  <rdfs:comment>Date of the instance. This implies "startDate" when a range is given with "endDate".</rdfs:comment>
  <rdfs:label>Date</rdfs:label>
</owl:DatatypeProperty>

<owl:DatatypeProperty rdf:about="#hasDepartmentCode">
  <rdfs:domain rdf:resource="#Course"/>
  <rdfs:range rdf:resource="http://www.w3.org/2001/XMLSchema#string"/>
  <rdfs:comment>Code of the department (this would imply that an organization is referenced too). For example: FIN, CFRM, FE, etc.</rdfs:comment>
  <rdfs:label>Department code</rdfs:label>
</owl:DatatypeProperty>

<owl:DatatypeProperty rdf:about="#hasImage">
  <rdfs:domain rdf:resource="#WorkExperience"/>
  <rdfs:range rdf:resource="http://www.w3.org/2001/XMLSchema#anyURI"/>
  <rdfs:comment>URL to image related to work experience. Can be used when displaying the information at consumption.</rdfs:comment>
  <rdfs:label>Image</rdfs:label>
</owl:DatatypeProperty>

<owl:DatatypeProperty rdf:about="#hasMedia">
  <rdfs:domain>
    <owl:Class>
      <owl:unionOf rdf:parseType="Collection">
        <rdf:Description rdf:about="#Accolade"/>
        <rdf:Description rdf:about="#ActivityType"/>
        <rdf:Description rdf:about="#Portfolio"/>
        <rdf:Description rdf:about="#WorkExperience"/>
      </owl:unionOf>
    </owl:Class>
  </rdfs:domain>
  <rdfs:range rdf:resource="http://www.w3.org/2001/XMLSchema#anyURI"/>
  <rdfs:comment>Additional media can be included here. For example, it could link to product/team pages, news articles, etc.</rdfs:comment>
  <rdfs:label>Media</rdfs:label>
</owl:DatatypeProperty>

<owl:DatatypeProperty rdf:about="#hasName">
  <rdfs:domain>
    <owl:Class>
      <owl:unionOf rdf:parseType="Collection">
        <rdf:Description rdf:about="#Accolade"/>
        <rdf:Description rdf:about="#ActivityType"/>
        <rdf:Description rdf:about="#Course"/>
        <rdf:Description rdf:about="#Degree"/>
        <rdf:Description rdf:about="#KnowledgeArea"/>
        <rdf:Description rdf:about="#Organization"/>
        <rdf:Description rdf:about="#Portfolio"/>
        <rdf:Description rdf:about="#SkillGroup"/>
        <rdf:Description rdf:about="#WorkExperience"/>
      </owl:unionOf>
    </owl:Class>
  </rdfs:domain>
  <rdfs:range rdf:resource="http://www.w3.org/2001/XMLSchema#string"/>
  <rdfs:comment>Human readable name for the entity; for display.</rdfs:comment>
  <rdfs:label>Human readable name</rdfs:label>
</owl:DatatypeProperty>

<owl:DatatypeProperty rdf:about="#hasPriority">
  <rdfs:domain rdf:resource="#Description"/>
  <rdfs:range rdf:resource="http://www.w3.org/2001/XMLSchema#nonNegativeInteger"/>
  <rdfs:comment>Priority level of the description (used for deciding truncation in toolkit). This is automatically set to the position of the string in the input "description" array of descriptions, when data is loaded using the command line tool.</rdfs:comment>
  <rdfs:label>description priority level</rdfs:label>
</owl:DatatypeProperty>

<owl:DatatypeProperty rdf:about="#hasStatus">
  <rdfs:domain rdf:resource="#Publication"/>
  <rdfs:range rdf:resource="http://www.w3.org/2001/XMLSchema#string"/>
  <rdfs:comment>Status of the publication. That is, this property should reflect a paper being "In Progress", or "Under Review".</rdfs:comment>
  <rdfs:label>Publication Status</rdfs:label>
</owl:DatatypeProperty>

<owl:DatatypeProperty rdf:about="#hasText">
  <rdfs:domain rdf:resource="#Description"/>
  <rdfs:range rdf:resource="http://www.w3.org/2001/XMLSchema#string"/>
  <rdfs:comment>Text of the description. This should be treated as a single "bullet point" on a traditional Resume/CV.</rdfs:comment>
  <rdfs:label>description text</rdfs:label>
</owl:DatatypeProperty>

<owl:DatatypeProperty rdf:about="#hasWebsite">
  <rdfs:domain>
    <owl:Class>
      <owl:unionOf rdf:parseType="Collection">
        <rdf:Description rdf:about="#Accolade"/>
        <rdf:Description rdf:about="#ActivityType"/>
        <rdf:Description rdf:about="#Course"/>
        <rdf:Description rdf:about="#Degree"/>
        <rdf:Description rdf:about="#Organization"/>
        <rdf:Description rdf:about="#Portfolio"/>
        <rdf:Description rdf:about="#SkillGroup"/>
        <rdf:Description rdf:about="#WorkExperience"/>
      </owl:unionOf>
    </owl:Class>
  </rdfs:domain>
  <rdfs:range rdf:resource="http://www.w3.org/2001/XMLSchema#anyURI"/>
  <rdfs:comment>External website of the entity (not used for ontology extension; treat this as user-facing).</rdfs:comment>
  <rdfs:label>Entity website</rdfs:label>
</owl:DatatypeProperty>

<owl:DatatypeProperty rdf:about="#inCity">
  <rdfs:domain>
    <owl:Class>
      <owl:unionOf rdf:parseType="Collection">
        <rdf:Description rdf:about="#Accolade"/>
        <rdf:Description rdf:about="#ActivityType"/>
        <rdf:Description rdf:about="#Course"/>
        <rdf:Description rdf:about="#Degree"/>
        <rdf:Description rdf:about="#Organization"/>
        <rdf:Description rdf:about="#Portfolio"/>
        <rdf:Description rdf:about="#SkillGroup"/>
        <rdf:Description rdf:about="#WorkExperience"/>
      </owl:unionOf>
    </owl:Class>
  </rdfs:domain>
  <rdfs:range rdf:resource="http://www.w3.org/2001/XMLSchema#string"/>
  <rdfs:comment>The city of the entity.</rdfs:comment>
  <rdfs:label>City</rdfs:label>
</owl:DatatypeProperty>

<owl:DatatypeProperty rdf:about="#inConferenceOrJournal">
  <rdfs:domain rdf:resource="#Publication"/>
  <rdfs:range rdf:resource="http://www.w3.org/2001/XMLSchema#string"/>
  <rdfs:comment>Conference/Journal name. This will eventually be replaced with a more semantically-correct representation of this information.</rdfs:comment>
  <rdfs:label>Conference/Journal Name</rdfs:label>
</owl:DatatypeProperty>

<owl:DatatypeProperty rdf:about="#inCountry">
  <rdfs:domain>
    <owl:Class>
      <owl:unionOf rdf:parseType="Collection">
        <rdf:Description rdf:about="#Accolade"/>
        <rdf:Description rdf:about="#ActivityType"/>
        <rdf:Description rdf:about="#Course"/>
        <rdf:Description rdf:about="#Organization"/>
        <rdf:Description rdf:about="#Portfolio"/>
        <rdf:Description rdf:about="#SkillGroup"/>
        <rdf:Description rdf:about="#WorkExperience"/>
      </owl:unionOf>
    </owl:Class>
  </rdfs:domain>
  <rdfs:range rdf:resource="http://www.w3.org/2001/XMLSchema#string"/>
  <rdfs:comment>Country of the entity.</rdfs:comment>
  <rdfs:label>Country</rdfs:label>
</owl:DatatypeProperty>

<owl:DatatypeProperty rdf:about="#inMonth">
  <rdfs:domain>
    <owl:Class>
      <owl:unionOf rdf:parseType="Collection">
        <rdf:Description rdf:about="#Accolade"/>
        <rdf:Description rdf:about="#ActivityType"/>
        <rdf:Description rdf:about="#Portfolio"/>
      </owl:unionOf>
    </owl:Class>
  </rdfs:domain>
  <rdfs:range rdf:resource="http://www.w3.org/2001/XMLSchema#int"/>
  <rdfs:comment>Month the portfolio item was completed.</rdfs:comment>
  <rdfs:label>Month of Portfolio Item</rdfs:label>
</owl:DatatypeProperty>

<owl:DatatypeProperty rdf:about="#inPublication">
  <rdfs:domain rdf:resource="#Publication"/>
  <rdfs:range rdf:resource="http://www.w3.org/2001/XMLSchema#string"/>
  <rdfs:comment>Publication name containing the specific publication. As with the other fields in the 'Publication' concept, this will probably be replaced eventually.</rdfs:comment>
  <rdfs:label>Publication Name</rdfs:label>
</owl:DatatypeProperty>

<owl:DatatypeProperty rdf:about="#inState">
  <rdfs:domain>
    <owl:Class>
      <owl:unionOf rdf:parseType="Collection">
        <rdf:Description rdf:about="#Accolade"/>
        <rdf:Description rdf:about="#ActivityType"/>
        <rdf:Description rdf:about="#Course"/>
        <rdf:Description rdf:about="#Degree"/>
        <rdf:Description rdf:about="#Organization"/>
        <rdf:Description rdf:about="#Portfolio"/>
        <rdf:Description rdf:about="#SkillGroup"/>
        <rdf:Description rdf:about="#WorkExperience"/>
      </owl:unionOf>
    </owl:Class>
  </rdfs:domain>
  <rdfs:range rdf:resource="http://www.w3.org/2001/XMLSchema#string"/>
  <rdfs:comment>State of the entity (United States only).</rdfs:comment>
  <rdfs:label>State</rdfs:label>
</owl:DatatypeProperty>

<owl:DatatypeProperty rdf:about="#inYear">
  <rdfs:domain>
    <owl:Class>
      <owl:unionOf rdf:parseType="Collection">
        <rdf:Description rdf:about="#Accolade"/>
        <rdf:Description rdf:about="#ActivityType"/>
        <rdf:Description rdf:about="#Portfolio"/>
      </owl:unionOf>
    </owl:Class>
  </rdfs:domain>
  <rdfs:range rdf:resource="http://www.w3.org/2001/XMLSchema#int"/>
  <rdfs:comment>Year the portfolio item was completed.</rdfs:comment>
  <rdfs:label>Year of Portfolio Item</rdfs:label>
</owl:DatatypeProperty>

<owl:DatatypeProperty rdf:about="#jobTitle">
  <rdfs:domain rdf:resource="#WorkExperience"/>
  <rdfs:range rdf:resource="http://www.w3.org/2001/XMLSchema#string"/>
  <rdfs:comment>Job Title for the work experience instance. Each work experience instance can have multiple job titles. For example, both "Software Engineering Intern" and "Software Engineer" could be job titles of the same work experience instance.</rdfs:comment>
  <rdfs:label>Job Title</rdfs:label>
</owl:DatatypeProperty>

<owl:DatatypeProperty rdf:about="#startDate">
  <rdfs:domain rdf:resource="#WorkExperience"/>
  <rdfs:range rdf:resource="http://www.w3.org/2001/XMLSchema#dateTime"/>
  <rdfs:comment>Start date of a WorkExperience.</rdfs:comment>
  <rdfs:label>Start date</rdfs:label>
</owl:DatatypeProperty>

<owl:DatatypeProperty rdf:about="#withGrade">
  <rdfs:domain rdf:resource="#Course"/>
  <rdfs:range>
    <rdfs:Datatype>
      <owl:onDatatype rdf:resource="http://www.w3.org/2001/XMLSchema#double"/>
      <owl:withRestrictions>
        <rdf:Description>
          <rdf:first>
            <rdf:Description>
              <xsd:minInclusive rdf:datatype="http://www.w3.org/2001/XMLSchema#double">0.0</xsd:minInclusive>
            </rdf:Description>
          </rdf:first>
          <rdf:rest>
            <rdf:Description>
              <rdf:first>
                <rdf:Description>
                  <xsd:maxInclusive rdf:datatype="http://www.w3.org/2001/XMLSchema#double">4.0</xsd:maxInclusive>
                </rdf:Description>
              </rdf:first>
              <rdf:rest rdf:resource="http://www.w3.org/1999/02/22-rdf-syntax-ns#nil"/>
            </rdf:Description>
          </rdf:rest>
        </rdf:Description>
      </owl:withRestrictions>
    </rdfs:Datatype>
  </rdfs:range>
  <rdfs:comment>Grade (GPA; 4.0 scale) received in the course (optional for obvious reasons :)).</rdfs:comment>
  <rdfs:label>Course GPA (on a 4.0 scale)</rdfs:label>
</owl:DatatypeProperty>

<owl:Class rdf:about="#Award">
  <rdfs:subClassOf rdf:resource="#Accolade"/>
  <rdfs:comment>An 'Award'; this would correspond to a traditional award, such as a Fellowship or Dean's List.</rdfs:comment>
  <rdfs:label>Award</rdfs:label>
</owl:Class>

<owl:Class rdf:about="#Certification">
  <rdfs:subClassOf rdf:resource="#Accolade"/>
  <rdfs:comment>A 'Cerficiation'; this would correspond to a traditional certification, such as a CPR Rating, or the Bloomberg Market Concepts certification.</rdfs:comment>
  <rdfs:label>Certification</rdfs:label>
</owl:Class>

<owl:Class rdf:about="#Project">
  <rdfs:subClassOf rdf:resource="#Portfolio"/>
  <rdfs:subClassOf>
    <owl:Restriction>
      <owl:onProperty rdf:resource="#hasCollaborators"/>
      <owl:someValuesFrom rdf:resource="http://www.w3.org/2001/XMLSchema#string"/>
    </owl:Restriction>
  </rdfs:subClassOf>
  <rdfs:comment>A project, such as a final year report, or a video produced for a class.</rdfs:comment>
  <rdfs:label>Project</rdfs:label>
</owl:Class>

<owl:Class rdf:about="#Talk">
  <rdfs:subClassOf rdf:resource="#Portfolio"/>
  <rdfs:subClassOf>
    <owl:Restriction>
      <owl:onProperty rdf:resource="#hasCollaborators"/>
      <owl:someValuesFrom rdf:resource="http://www.w3.org/2001/XMLSchema#string"/>
    </owl:Restriction>
  </rdfs:subClassOf>
  <rdfs:subClassOf>
    <owl:Restriction>
      <owl:onProperty rdf:resource="#hasDate"/>
      <owl:onDataRange rdf:resource="http://www.w3.org/2001/XMLSchema#dateTime"/>
      <owl:minQualifiedCardinality rdf:datatype="http://www.w3.org/2001/XMLSchema#nonNegativeInteger">1</owl:minQualifiedCardinality>
    </owl:Restriction>
  </rdfs:subClassOf>
  <rdfs:comment>A talk or presentation.</rdfs:comment>
  <rdfs:label>Talk</rdfs:label>
</owl:Class>

<Organization rdf:about="http://rukmal.me/precis/musk#spacex">
  <rdf:type rdf:resource="http://www.w3.org/2002/07/owl#NamedIndividual"/>
  <externalResource rdf:datatype="http://www.w3.org/2001/XMLSchema#string">http://dbpedia.org/resource/SpaceX</externalResource>
  <hasName rdf:datatype="http://www.w3.org/2001/XMLSchema#string">Space Exploration Technologies Corporation</hasName>
  <hasWebsite rdf:datatype="http://www.w3.org/2001/XMLSchema#string">https://www.spacex.com/</hasWebsite>
</Organization>

<Description rdf:about="http://rukmal.me/precis/musk#3ea2ff88-f7bf-4b05-a906-4ace6f095ed4">
  <rdf:type rdf:resource="http://www.w3.org/2002/07/owl#NamedIndividual"/>
  <hasPriority rdf:datatype="http://www.w3.org/2001/XMLSchema#integer">1</hasPriority>
  <hasText rdf:datatype="http://www.w3.org/2001/XMLSchema#string">Launched SpaceX.</hasText>
</Description>

<Description rdf:about="http://rukmal.me/precis/musk#c202157f-de48-487b-bfcc-a632447d6299">
  <rdf:type rdf:resource="http://www.w3.org/2002/07/owl#NamedIndividual"/>
  <hasPriority rdf:datatype="http://www.w3.org/2001/XMLSchema#integer">2</hasPriority>
  <hasText rdf:datatype="http://www.w3.org/2001/XMLSchema#string">Led the development of the first commercially viable reusable orbital class rocket.</hasText>
</Description>

<WorkExperience rdf:about="http://rukmal.me/precis/musk#we_spacex_ceo">
  <rdf:type rdf:resource="http://www.w3.org/2002/07/owl#NamedIndividual"/>
  <employedAt rdf:resource="http://rukmal.me/precis/musk#spacex"/>
  <hasDescription rdf:resource="http://rukmal.me/precis/musk#3ea2ff88-f7bf-4b05-a906-4ace6f095ed4"/>
  <hasDescription rdf:resource="http://rukmal.me/precis/musk#c202157f-de48-487b-bfcc-a632447d6299"/>
  <hasDate rdf:datatype="http://www.w3.org/2001/XMLSchema#dateTime">2002-05-01T00:00:00</hasDate>
  <hasImage rdf:datatype="http://www.w3.org/2001/XMLSchema#string"></hasImage>
  <inCity rdf:datatype="http://www.w3.org/2001/XMLSchema#string">Hawthorne</inCity>
  <inState rdf:datatype="http://www.w3.org/2001/XMLSchema#string">CA</inState>
  <jobTitle rdf:datatype="http://www.w3.org/2001/XMLSchema#string">Founder, CEO and Lead Designer</jobTitle>
</WorkExperience>

<Organization rdf:about="http://rukmal.me/precis/musk#tesla">
  <rdf:type rdf:resource="http://www.w3.org/2002/07/owl#NamedIndividual"/>
  <externalResource rdf:datatype="http://www.w3.org/2001/XMLSchema#string">http://dbpedia.org/resource/Tesla_Motors</externalResource>
  <hasName rdf:datatype="http://www.w3.org/2001/XMLSchema#string">Tesla Motors</hasName>
  <hasWebsite rdf:datatype="http://www.w3.org/2001/XMLSchema#string">https://www.tesla.com/</hasWebsite>
</Organization>

<WorkExperience rdf:about="http://rukmal.me/precis/musk#we_tesla_ceo">
  <rdf:type rdf:resource="http://www.w3.org/2002/07/owl#NamedIndividual"/>
  <employedAt rdf:resource="http://rukmal.me/precis/musk#tesla"/>
  <hasDate rdf:datatype="http://www.w3.org/2001/XMLSchema#dateTime">2003-01-01T00:00:00</hasDate>
  <hasImage rdf:datatype="http://www.w3.org/2001/XMLSchema#string"></hasImage>
  <inCity rdf:datatype="http://www.w3.org/2001/XMLSchema#string">San Mateo</inCity>
  <inState rdf:datatype="http://www.w3.org/2001/XMLSchema#string">CA</inState>
  <jobTitle rdf:datatype="http://www.w3.org/2001/XMLSchema#string">CEO and Product Architect</jobTitle>
</WorkExperience>

<Description rdf:about="http://rukmal.me/precis/musk#cf9631c0-44d7-44e4-aae2-02c82e292b1a">
  <rdf:type rdf:resource="http://www.w3.org/2002/07/owl#NamedIndividual"/>
  <hasPriority rdf:datatype="http://www.w3.org/2001/XMLSchema#integer">0</hasPriority>
  <hasText rdf:datatype="http://www.w3.org/2001/XMLSchema#string">Given to people who have rendered meritorious service to humanity in the IEEE's designated fields of interest.</hasText>
</Description>

<Award rdf:about="http://rukmal.me/precis/musk#award:ieee">
  <rdf:type rdf:resource="http://www.w3.org/2002/07/owl#NamedIndividual"/>
  <affiliatedWith rdf:resource="http://rukmal.me/precis/musk#we_tesla_ceo"/>
  <hasDescription rdf:resource="http://rukmal.me/precis/musk#cf9631c0-44d7-44e4-aae2-02c82e292b1a"/>
  <externalResource rdf:datatype="http://www.w3.org/2001/XMLSchema#string">http://dbpedia.org/resource/IEEE_Honorary_Membership</externalResource>
  <hasName rdf:datatype="http://www.w3.org/2001/XMLSchema#string">IEEE Honorary Membership</hasName>
  <inYear rdf:datatype="http://www.w3.org/2001/XMLSchema#string">2015</inYear>
</Award>

<Organization rdf:about="http://rukmal.me/precis/musk#org_upenn">
  <rdf:type rdf:resource="http://www.w3.org/2002/07/owl#NamedIndividual"/>
  <hasName rdf:datatype="http://www.w3.org/2001/XMLSchema#string">University of Pennsylvania</hasName>
  <hasWebsite rdf:datatype="http://www.w3.org/2001/XMLSchema#string">https://www.upenn.edu/</hasWebsite>
</Organization>

<Organization rdf:about="http://rukmal.me/precis/musk#org_upenn_wharton">
  <rdf:type rdf:resource="http://www.w3.org/2002/07/owl#NamedIndividual"/>
  <hasParentOrganization rdf:resource="http://rukmal.me/precis/musk#org_upenn"/>
  <hasName rdf:datatype="http://www.w3.org/2001/XMLSchema#string">Wharton School</hasName>
  <hasWebsite rdf:datatype="http://www.w3.org/2001/XMLSchema#string">https://www.wharton.upenn.edu/</hasWebsite>
</Organization>

<Organization rdf:about="http://rukmal.me/precis/musk#org_upenn_wharton_econ">
  <rdf:type rdf:resource="http://www.w3.org/2002/07/owl#NamedIndividual"/>
  <hasParentOrganization rdf:resource="http://rukmal.me/precis/musk#org_upenn_wharton"/>
  <hasName rdf:datatype="http://www.w3.org/2001/XMLSchema#string">Department of Business Economics and Public Policy</hasName>
  <hasWebsite rdf:datatype="http://www.w3.org/2001/XMLSchema#string">https://bepp.wharton.upenn.edu/</hasWebsite>
</Organization>

<Degree rdf:about="http://rukmal.me/precis/musk#degree_bs_econ">
  <rdf:type rdf:resource="http://www.w3.org/2002/07/owl#NamedIndividual"/>
  <degreeUniversity rdf:resource="http://rukmal.me/precis/musk#org_upenn"/>
  <degreeDepartment rdf:resource="http://rukmal.me/precis/musk#org_upenn_wharton_econ"/>
  <degreeSchool rdf:resource="http://rukmal.me/precis/musk#org_upenn_wharton"/>
  <degreeConcentration rdf:datatype="http://www.w3.org/2001/XMLSchema#string">http://dbpedia.org/resource/Economics</degreeConcentration>
  <degreeType rdf:datatype="http://www.w3.org/2001/XMLSchema#string">http://dbpedia.org/resource/Bachelor_of_Science</degreeType>
  <hasDate rdf:datatype="http://www.w3.org/2001/XMLSchema#dateTime">1995-06-01T00:00:00</hasDate>
  <hasName rdf:datatype="http://www.w3.org/2001/XMLSchema#string">Bachelor of Science in Economics</hasName>
  <inCity rdf:datatype="http://www.w3.org/2001/XMLSchema#string">Philadephia</inCity>
  <inState rdf:datatype="http://www.w3.org/2001/XMLSchema#string">PA</inState>
</Degree>

<Organization rdf:about="http://rukmal.me/precis/musk#org_upenn_sas">
  <rdf:type rdf:resource="http://www.w3.org/2002/07/owl#NamedIndividual"/>
  <hasParentOrganization rdf:resource="http://rukmal.me/precis/musk#org_upenn"/>
  <hasName rdf:datatype="http://www.w3.org/2001/XMLSchema#string">School of Arts and Science</hasName>
  <hasWebsite rdf:datatype="http://www.w3.org/2001/XMLSchema#string">https://www.sas.upenn.edu/</hasWebsite>
</Organization>

<Organization rdf:about="http://rukmal.me/precis/musk#org_upenn_physics">
  <rdf:type rdf:resource="http://www.w3.org/2002/07/owl#NamedIndividual"/>
  <hasParentOrganization rdf:resource="http://rukmal.me/precis/musk#org_upenn_sas"/>
  <hasName rdf:datatype="http://www.w3.org/2001/XMLSchema#string">Department of Physics and Astronomy</hasName>
  <hasWebsite rdf:datatype="http://www.w3.org/2001/XMLSchema#string">https://www.physics.upenn.edu/</hasWebsite>
</Organization>

<Degree rdf:about="http://rukmal.me/precis/musk#degree_bs_physics">
  <rdf:type rdf:resource="http://www.w3.org/2002/07/owl#NamedIndividual"/>
  <degreeUniversity rdf:resource="http://rukmal.me/precis/musk#org_upenn"/>
  <degreeDepartment rdf:resource="http://rukmal.me/precis/musk#org_upenn_physics"/>
  <degreeSchool rdf:resource="http://rukmal.me/precis/musk#org_upenn_sas"/>
  <degreeConcentration rdf:datatype="http://www.w3.org/2001/XMLSchema#string">http://dbpedia.org/resource/Physics</degreeConcentration>
  <degreeType rdf:datatype="http://www.w3.org/2001/XMLSchema#string">http://dbpedia.org/resource/Bachelor_of_Science</degreeType>
  <hasDate rdf:datatype="http://www.w3.org/2001/XMLSchema#dateTime">1995-06-01T00:00:00</hasDate>
  <hasName rdf:datatype="http://www.w3.org/2001/XMLSchema#string">Bachelor of Science in Physics</hasName>
  <inCity rdf:datatype="http://www.w3.org/2001/XMLSchema#string">Philadelphia</inCity>
  <inState rdf:datatype="http://www.w3.org/2001/XMLSchema#string">PA</inState>
</Degree>

<Project rdf:about="http://rukmal.me/precis/musk#proj_spacex_falcon_heavy">
  <rdf:type rdf:resource="http://www.w3.org/2002/07/owl#NamedIndividual"/>
  <affiliatedWith rdf:resource="http://rukmal.me/precis/musk#we_spacex_ceo"/>
  <externalResource rdf:datatype="http://www.w3.org/2001/XMLSchema#string">http://dbpedia.org/resource/Falcon_Heavy</externalResource>
  <hasDate rdf:datatype="http://www.w3.org/2001/XMLSchema#dateTime">2018-02-06T00:00:00</hasDate>
  <hasWebsite rdf:datatype="http://www.w3.org/2001/XMLSchema#string">https://www.spacex.com/falcon-heavy</hasWebsite>
</Project>

<Publication rdf:about="http://rukmal.me/precis/musk#proj_spacex_hyperloop_alpha">
  <rdf:type rdf:resource="http://www.w3.org/2002/07/owl#NamedIndividual"/>
  <affiliatedWith rdf:resource="http://rukmal.me/precis/musk#we_spacex_ceo"/>
  <externalResource rdf:datatype="http://www.w3.org/2001/XMLSchema#string">http://dbpedia.org/resource/Hyperloop</externalResource>
  <hasDate rdf:datatype="http://www.w3.org/2001/XMLSchema#dateTime">2013-08-16T00:00:00</hasDate>
  <hasWebsite rdf:datatype="http://www.w3.org/2001/XMLSchema#string">https://www.spacex.com/sites/spacex/files/hyperloop_alpha.pdf</hasWebsite>
</Publication>

<owl:AllDisjointClasses>
  <owl:members rdf:parseType="Collection">
    <rdf:Description rdf:about="#Accolade"/>
    <rdf:Description rdf:about="#ActivityType"/>
    <rdf:Description rdf:about="#Course"/>
    <rdf:Description rdf:about="#Degree"/>
    <rdf:Description rdf:about="#Description"/>
    <rdf:Description rdf:about="#KnowledgeArea"/>
    <rdf:Description rdf:about="#Organization"/>
    <rdf:Description rdf:about="#Portfolio"/>
    <rdf:Description rdf:about="#SkillGroup"/>
    <rdf:Description rdf:about="#WorkExperience"/>
  </owl:members>
</owl:AllDisjointClasses>

<owl:Axiom>
  <owl:annotatedSource rdf:resource="#Organization"/>
  <owl:annotatedProperty rdf:resource="http://www.w3.org/2000/01/rdf-schema#subClassOf"/>
  <owl:annotatedTarget>
    <owl:Restriction>
      <owl:onProperty rdf:resource="#hasDescription"/>
      <owl:onClass rdf:resource="#Description"/>
      <owl:maxQualifiedCardinality rdf:datatype="http://www.w3.org/2001/XMLSchema#nonNegativeInteger">1</owl:maxQualifiedCardinality>
    </owl:Restriction>
  </owl:annotatedTarget>
  <rdfs:comment>This should be used to add an additional descriptive string if necessary. For example, this could be a team name or a descriptive string (eg: "Startup Company", etc.).</rdfs:comment>
</owl:Axiom>


</rdf:RDF>
